Work in progress

TM/Combinators/While.v
@@ -6,38 +6,38 @@ Section While.
   Variable n : nat.
   Variable sig : finType.
 
-  Variable M : mTM sig n.
-
-  Variable p : states M -> bool.
+  Variable pM : { M : mTM sig n & states M -> bool }.
   
   Definition while_trans :
-    (TM.states M) * Vector.t (option sig) n ->
-    (TM.states M) * Vector.t (option sig * move) n :=
+    (TM.states (projT1 pM)) * Vector.t (option sig) n ->
+    (TM.states (projT1 pM)) * Vector.t (option sig * move) n :=
     fun st => let (s,a) := st in
-           if p s && halt s then (start M,null_action) else trans st.
+           if projT2 pM s && halt s then (start (projT1 pM),null_action) else trans st.
 
   Definition While : mTM sig n :=
-    Build_mTM while_trans (start M)
-              (fun s => halt s && negb (p s)).
+    Build_mTM while_trans (start (projT1 pM))
+              (fun s => halt s && negb (projT2 pM s)).
+
+  Definition WHILE := (While; fun _ => tt).
 
   Local Arguments loopM {_ _} _ _ _.
   Local Arguments halt {_ _} _ _.
   Local Arguments step {_ _} _ _.
 
 
-  Definition unlift_1 : mconfig sig (states While) n -> option (mconfig sig (states M) n).
+  Definition unlift_1 : mconfig sig (states While) n -> option (mconfig sig (states (projT1 pM)) n).
   Proof.
-    intros s. exact (if (halt M (cstate s)) then Some s else None).
+    intros s. exact (if (halt (projT1 pM) (cstate s)) then Some s else None).
   Defined.
  
   Lemma While_split i res c:
     loopM While i c = Some res ->
-    (exists i1 x1 i2,  loopM M i1 c = Some x1 /\
+    (exists i1 x1 i2,  loopM (projT1 pM) i1 c = Some x1 /\
                      loopM While i2 x1 = Some res /\ i = i1 + i2 ).
   Proof.
     intros.
     unfold loopM in H.
-    eapply loop_split with (p := fun c=> halt M (cstate c)) in H.
+    eapply loop_split with (p := fun c=> halt (projT1 pM) (cstate c)) in H.
     destruct H as (i1 & x1 & i2 & H1 & H2 & ->).
     -exists i1,x1,i2. split;[ |split;[exact H2|reflexivity]].
      eapply loop_lift with (lift:=id) in H1.
@@ -48,12 +48,12 @@ Section While.
   Qed.
 
   Lemma While_true_split i (x : mconfig _ (states While) _) oenc :
-    halt M (cstate x) = true  -> p (cstate x) = true->
+    halt (projT1 pM) (cstate x) = true  -> projT2 pM (cstate x) = true->
     loopM While i x = Some oenc ->
     exists i', i = 1+i' /\ loopM While i' (initc While (ctapes x)) = Some oenc.
   Proof.
     intros hx px Eq.
-    destruct i as [ |i'];cbn in Eq;cbn in Eq; change (states M) with (states While) in Eq; rewrite hx,px in Eq;cbn in Eq; inv Eq.
+    destruct i as [ |i'];cbn in Eq;cbn in Eq; change (states (projT1 pM)) with (states While) in Eq; rewrite hx,px in Eq;cbn in Eq; inv Eq.
     exists i'. split;[omega| ].
     destruct x. cbn in *. rewrite <- H0. unfold loopM. f_equal.
     unfold step. cbn -[tape_move_multi null_action]. 
@@ -61,31 +61,29 @@ Section While.
   Qed.
 
   Lemma While_true_merge i1 i2 (t x1 : mconfig _ (states While) _) oenc :
-    loopM M i1 t = Some x1 ->
+    loopM (projT1 pM) i1 t = Some x1 ->
     loopM While i2 (initc While (ctapes x1)) = Some oenc ->
-    p (cstate x1) = true ->
+    (projT2 pM) (cstate x1) = true ->
     loopM While (i1+(1+i2)) t = Some oenc.
   Proof.
     intros Eq1 Eq2 px1.
     eapply loop_merge with
-    (p:= fun c => halt M (cstate c)) (a2:=x1).
+    (p:= fun c => halt (projT1 pM) (cstate c)) (a2:=x1).
     {unfold While. cbn. intros. now destruct halt. }
-    {change (states While) with (states M) in *.
+    {change (states While) with (states (projT1 pM)) in *.
      eapply loop_lift with (g:= step While) in Eq1;[exact Eq1|reflexivity| ].
      intros. unfold step,While,while_trans. cbn. now rewrite H,andb_false_r.
     }
-    cbn. assert (hx1:halt M (cstate x1)=true) by (apply loop_fulfills_p in Eq1;now destruct halt).
-    change (states While) with (states M) in *.
+    cbn. assert (hx1:halt (projT1 pM) (cstate x1)=true) by (apply loop_fulfills_p in Eq1;now destruct halt).
+    change (states While) with (states (projT1 pM)) in *.
     rewrite hx1;cbn.
-    -rewrite <- Eq2. unfold loopM. cbn. f_equal. unfold step. cbn -[tape_move_multi null_action].  rewrite hx1,px1;cbn -[tape_move_multi null_action]. now rewrite tape_move_null_action. 
-    (*-unfold loopM in Eq2. erewrite loop_fulfills_p_0 in Eq2;cbn. destruct x1;cbn in *. inv Eq2.
-     f_equal. unfold initc. repeat f_equal. unfold initc in Eq2. cbn in Eq2. inv Eq2. f_equal. eapply loop_functional. inSearchAbout loop. unfold loop
-      *)
+    -rewrite <- Eq2. unfold loopM. cbn. f_equal. unfold step. cbn -[tape_move_multi null_action].
+     rewrite hx1,px1;cbn -[tape_move_multi null_action]. now rewrite tape_move_null_action. 
   Qed.
 
    Lemma While_false_merge i1 (t : mconfig _ (states While) _) oenc :
-    loopM M i1 t = Some oenc ->
-    p (cstate oenc) = false ->
+    loopM (projT1 pM) i1 t = Some oenc ->
+    projT2 pM (cstate oenc) = false ->
     loopM While i1 t = Some oenc.
   Proof.
     intros Eq px1.
@@ -93,7 +91,7 @@ Section While.
       in Eq. destruct Eq as (?&H'&H1). inv H1.
     Focus 3. intros ? ? H. inv H. reflexivity.
     replace i1 with (i1+0) by omega.
-    eapply (loop_merge (p:= fun c => halt M (cstate c))). unfold halt at 2. cbn. 
+    eapply (loop_merge (p:= fun c => halt (projT1 pM) (cstate c))). unfold halt at 2. cbn. 
     now intros ? ->. exact H'.
     apply loop_fulfills_p_0. unfold halt. cbn. rewrite px1.
     apply loop_fulfills_p in H'. now destruct halt.
@@ -101,16 +99,16 @@ Section While.
     cbn in H0. f_equal. unfold step at 2;cbn. rewrite H0. now rewrite andb_false_r.  reflexivity. 
   Qed.
     
-  Lemma While_sem (R : Rel _ (bool * _)) :
-    M ⊫(p) R ->
-    While ⊫(fun _ => tt) ( (star (R |_ true)) ∘ (ignoreParam (R |_ false))).
+  Lemma While_Realise (R : Rel _ (bool * _)) :
+    pM ⊫ R ->
+    WHILE ⊫ ( (star (R |_ true)) ∘ (ignoreParam (R |_ false))).
   Proof.
     intros HR t1 i1 oenc2 eq. unfold initc in eq.
-    revert t1 eq;apply complete_induction with (x:=i1). clear i1; intros i1 IH t1 eq.
+    revert t1 eq; apply complete_induction with (x:=i1); clear i1; intros i1 IH t1 eq.
     apply While_split in eq as (i2&x0&i3&Eq1&Eq2&->).
-    assert (hx0 : halt M (cstate x0) = true)
+    assert (hx0 : halt (projT1 pM) (cstate x0) = true)
       by (eapply loop_fulfills_p in Eq1;  destruct halt;auto).
-    destruct (p (cstate x0)) eqn: px0.
+    destruct (projT2 pM (cstate x0)) eqn: px0.
     -apply While_true_split in Eq2 as (i' & -> & Eq2);[ |assumption..].
      apply IH in Eq2;[ |omega].
      eapply use_subrel.
@@ -123,15 +121,58 @@ Section While.
      unfold loopM in Eq2; rewrite loop_fulfills_p_0 in Eq2;[ |cbn;now rewrite hx0, px0]. inv Eq2.
      apply HR in Eq1. cbn in Eq1. now rewrite px0 in Eq1.
   Qed.
+
+
+  (*
+  (* TODO Versuche erst das zu beweisen und daraus das induktive Ding unten zu zeigen *)
+  Lemma While_terminatesIn' t :
+
+    pM ↓(T) ->
+    (forall (x : tapes sig n) '(y, i),
+        T' x (y, i) -> exists (x':tapes _ _) (b:bool) i1 y1,
+           T x (y1,i1) /\ if b then exists i2 y2, T' x' (y2, i2) /\ i1+1+i2<=i else i1 <= i)->
+    WHILE ↓(T').
+  Proof.
+    intros Term_M Hyp. hnf.
+    intros t i. revert t. apply complete_induction with (x:=i); clear i; intros i IH t T't.
+    destruct (Hyp _ _ T't) as (t'& b& i1&Rx&Tx&H).
+    destruct b.
+    -destruct H as (i2&T't'&Leq).
+     apply IH in T't' as (oenc & Eq);[ |omega].
+     exists oenc.
+     apply Term_M in Tx as (oenc1 & Eq1).
+     apply (loop_ge (k1:=i1 + (1 + i2)));[omega| ].
+     specialize (HR _ _ _ Eq1). specialize (Func _ _ T't _ _ HR Rx). inv Func.
+     now apply (While_true_merge Eq1).
+    -apply Term_M in Tx as [oenc Eq].
+     exists oenc.
+     eapply While_false_merge. eapply loop_ge;[ |exact Eq]. omega.
+     specialize (HR _ _ _ Eq).
+     specialize (Func _ _ T't _ _ HR Rx). now inv Func.
+  Qed.
+*)
+
+  (*
+  Section WhileTerm.
+
+    Inductive WhileTerm : Rel (tapes sig n) (unit * nat) :=
+    | term_false input i          : T input (false, i) -> WhileTerm input (tt, i)
+    | term_true  input i j output : T input (true,  i) -> WhileTerm output (tt, j) -> WhileTerm input (tt, i+1+j).
+
+  End WhileTerm.
   
-  Lemma While_terminatesIn (R : Rel _ (bool * _)) (T T': Rel _ nat):
-    M ⊫(p) R ->
-    M ↓(T) ->
-    functionalOn T' R -> 
-    (forall (x : tapes sig n) (i:nat),
-        T' x i -> exists (x':tapes _ _) (b:bool) i1,
-          R x (b,x') /\ T x i1 /\ if b then exists i2, T' x' i2 /\ i1+1+i2<=i else i1 <= i)->
-    While ↓(T').
+  
+  Lemma While_Terminates (T : Rel _ (_ * nat)):
+    pM ↓(T) -> WHILE ↓(WhileTerm T).
+  Proof.
+    intros Term. hnf. intros t1. specialize (Term t1) as (c1&i1&eq&Term).
+    revert t1 eq Term; apply complete_induction with (x:=i1); clear i1; intros i1 IH t1 eq Term.
+    destruct c1 as [b tapes1].
+    destruct (
+
+
+
+  Restart.
   Proof.
     intros HR Term_M Func Hyp.
     intros t i. revert t. apply complete_induction with (x:=i); clear i; intros i IH t T't.
@@ -150,17 +191,7 @@ Section While.
      specialize (HR _ _ _ Eq).
      specialize (Func _ _ T't _ _ HR Rx). now inv Func.
   Qed.
+*)
 
 End While.
-Arguments While {n} {sig} M _.
-
-Section While_total.
-
-  Variable n : nat.
-  Variable sig : finType.
-
-  Variable pM : { M : mTM sig n & states M -> bool}.
-
-  Definition WHILE := (While (projT1 pM) (projT2 pM) ; fun _ => tt).
-
-End While_total.
+(* Arguments While {n} {sig} M _. *)
